elm-letrec-test/src/TopMutualRec.elm
@@ -1,0 +1,30 @@
+module TopMutualRec exposing (main)
+
+-- Top-level version of MutualRec, to compare let vs top-level behaviour.
+
+import Html
+
+
+even2 : List a -> Int
+even2 xs =
+    case xs of
+        [] ->
+            0
+
+        _ :: rest ->
+            odd2 [ rest ]
+
+
+odd2 : List a -> Int
+odd2 xs =
+    case xs of
+        [] ->
+            1
+
+        _ :: rest ->
+            even2 rest
+
+
+main : Html.Html msg
+main =
+    Html.text (String.fromInt (even2 [ 1, 2, 3 ]))
